$0,1,2,\dots$ 
$\omega=sup \{ 0,1,2,\dots \}$ 
Next one is $\omega^{+}$ which we will write as $\omega+1$ (for now, just notation)
Continue: $\omega+2,\omega+3,\dots$ and then 
$sup \{ \omega+n :n<\omega\}=\omega+\omega=\omega \cdot 2$
Then continue with 
$\omega \cdot 2+1,\omega \cdot 2+2,\dots,\omega \cdot 3$
So get 
$\omega,\omega \cdot 2,\omega \cdot 3,\dots \omega \cdot \omega=\omega^{2}$
Then get $\omega^{2}\cdot 2,\omega^{2} \cdot 3,\dots \omega^{2}\cdot \omega=\omega^{3}$
So have
$\omega,\omega^{2},\omega^{3},\dots,\omega^{\omega}$
Eventually, get 
$\omega^{\omega }\cdot 2\dots \omega^{\omega+1}\dots \omega^{\omega^{2}}\dots \omega^{\omega^{\omega}}\dots$