We consider the diffusion equation
$$
\frac{\partial u}{\partial t} = \frac{\partial^{2}u}{\partial x^{2}}
$$
where $-\infty<x<\infty$ and $t\geq 0$
We assume a recurrence of the form:
$$
\sum_{k=r}^{s}a_{k}u_{m+k}^{n+1}=\sum_{k=r}^{s}b_{k}u_{m+k}^{n}
$$
where $m\in \mathbb{Z}$
## Fourier analysis of stability
[[Fourier Analysis of Stability]]
### Euler
$$
u_{m}^{n+1} = u_{m}^{n} + \mu(u_{m-1}^{n}-2u_{m}^{n}+u_{m+1}^{n})
$$
has amplification factor:
$$
H(\theta) = 1+\mu(e^{-i\theta}-2+e^{i\theta}) = 1- 4\mu \sin ^{2} \frac{\theta}{2} \in [1-4\mu,1]
$$
this the method is stable iff $\mu\leq \frac{1}{2}$
### Reverse Euler
$$
u_{m}^{n+1}-\mu(u_{m-1}^{n+1}-2u_{m}^{n+1}+u_{m+1}^{n+1}) = u_{m}^{n}
$$
has amp:
$$
H(\theta) = (1-\mu(e^{-i\theta}-2+e^{i\theta}))^{-1} = \left( 1+4\mu \sin ^{2} \frac{\theta}{2} \right)^{-1} \in(0,1]
$$
thus is stable for all $\mu>0$
### Crank-Nicolson
$$
u_{m}^{n+1}-\frac{1}{2}\mu(u_{m-1}^{n+1}-2u_{m}^{n+1}+u_{m+1}^{n+1}) = u_{m}^{n} +\frac{1}{2} \mu(u_{m-1}^{n}-2u_{m}^{n}+u_{m+1}^{n})
$$
has amp:
$$
H(\theta) = \frac{1+\frac{1}{2}\mu(e^{-i\theta}-2+e^{i\theta})}{1-\frac{1}{2}\mu(e^{-i\theta}-2+e^{i\theta})}
=\frac{1-2\mu \sin ^{2} \frac{\theta}{2}}{1+2\mu \sin ^{2} \frac{\theta}{2}}
\in(-1,1]
$$
So stable for all $\mu>0$